providers/quic/Spec.QUIC.fsti
@@ -117,7 +117,11 @@ val lemma_header_parsing_correct: h:header -> pn_len:nat2 -> npn:lbytes (1+pn_le
 
 // N.B. this is only true for a given DCID len
 val lemma_header_parsing_safe: b1:bytes -> b2:bytes -> cl:nat4 -> Lemma
-  (parse_header b1 cl == parse_header b2 cl ==> b1 == b2)
+  (requires
+    H_Success? (parse_header b1 cl) /\
+    H_Success? (parse_header b2 cl) /\
+    parse_header b1 cl == parse_header b2 cl)
+  (ensures b1 == b2)
 
 // Header protection only
 val header_encrypt: a:ea ->
